\section{Problem 1}~\label{sec:prob1}

\subsection{} % 1.1

\begin{equation}
\begin{split}
    P(\vx)
        &= \sum_h \frac{e^{-E(\vx,\vh)}}{Z} \\
        &= \exp\bigg(\log\sum_h\frac{e^{-E(\vx,\vh)}}{Z}\bigg) \\
        &= \exp\bigg(\log\sum_h e^{-E(\vx,\vh)} - \log Z\bigg) \\
        &= \frac{\exp\bigg(\log\sum_h e^{-E(\vx,\vh)}\bigg)}{Z} \\
        &= \frac{e^{-\cF(\vx)}}{Z}. \\
\end{split}
\end{equation}

\subsection{} % 1.2

\begin{equation}
\begin{split}
    -\frac{\partial\log p(\vx)}{\partial\theta}
        &= -\frac{\partial}{\partial\theta}\log\bigg(\frac{e^{-\cF(\vx)}}{Z}\bigg) \\
        &= -\frac{\partial(-\cF(\vx))}{\partial\theta} + \frac{\partial \log Z}{\partial\theta} \\
        &= \frac{\partial \cF(\vx)}{\partial\theta} + \frac{1}{Z}\frac{\partial}{\partial\theta} \sum_{\tilde\vx} e^{-\cF(\tilde\vx)}\\
        &= \frac{\partial \cF(\vx)}{\partial\theta} - \sum_{\tilde\vx} \frac{\partial\cF(\tilde\vx)}{\partial\theta}\frac{e^{-\cF(\tilde\vx)}}{Z}\\
        &= \frac{\partial \cF(\vx)}{\partial\theta} - \sum_{\tilde\vx} \frac{\partial\cF(\tilde\vx)}{\partial\theta}p(\tilde\vx)\\
\end{split}
\end{equation}

\subsection{} % 1.3
